\documentclass{article}
\usepackage{amsmath,amssymb, amsthm}
\begin{document}
%	\begin{align}
%		\intertext{Distance between Solwezi and Lusaka:}
%		distance &= 1500km \\
%		\intertext{Given, the relation between miles and kilometer is:}
%		mile &= 1.61km \\
%		distance\_in\_miles &= distance/miles
%		%LHS &= (2x+5y)^2 - (2x-5y)^2 \\
%		%\text{or, } LHS &= \{(2x+5y) + (2x-5y)\}\{(2x+5y) - (2x-5y)\} \\
%		%\text{or, } LHS &= \{(4x)\}\{(10y)\}\\
%		%\text{or, } LHS &= 20xy
%		\intertext{Compound amount earned by $A$ after $t=2$ years is equal to the Compound amount earned by $B$ after $t=3$ years.}
%		x\left(1+\frac{4}{100}\right)^2 &= (81600-x)\left(1 + \frac{4}{100}\right)^3 \nonumber\\
%		\text{or, } x &= (81600 - x)(1.04) \nonumber\\
%		\text{or, } x(1+1.04) &= 81600(1.04) \nonumber\\
%		\text{or, } x &= \frac{81600*1.04}{2.04} \nonumber\\
%		\text{or, } x &= 41600 \nonumber		
%	\end{align}

\section{Question 01}
Prove that if $a, b \text{ and } c$ form a Pythagorean triplet i.e. $a^2 + b^2 = c^2$, then $ka, kb \text{ and } kc$ also form a Pythagorean triplet where $k$ is a real positive constant.

\begin{align}
	\intertext{Given, } a^2+ b^2 = c^2 \label{eq:given01}\\
	\intertext{To prove that:}
	(ka)^2 + (kb)^2 = (kc)^2 \label{eq:tpt01}
	\intertext{Starting with the LHS of \ref{eq:tpt01}:}
	LHS = (ka)^2 + (kb)^2 \nonumber\\
	\text{or, } LHS = k^2 a^2 + k^2 b^2 \nonumber\\
	\text{or, } LHS = k^2(a^2 + b^2) \nonumber\\
	\intertext{But from \ref{eq:given01}, we know that} a^2 + b^2 = c^2 \nonumber\\
	\text{which makes } LHS = k^2c^2 \nonumber
	\intertext{which is what we set out to prove.}
	\intertext{Therefore if $a, b, \text{ and } c$ form a Pythagorean triplet then so do $ka, kb \text{ and } kc$. Hence Proved.}  	
\end{align}
\end{document}