\section{Problem 3}
Consider any uncertain experiment, and let $A$, $B$, and $C$ be three events defined for the experiment. Please prove the following equalities or inequalities. In doing so, you may use the three axioms, any equalities/inequalities developed in class, standard set theory and algebra concepts, and earlier parts of the problem.

\begin{enumerate}[a.]
	\item
	\!  %one-sixth of a quad's space, the Stack Exchange answer did this so I'm doing the same too.
	$
	\begin{aligned}
		P(A\bar B) = P(A) -  P(AB) \nonumber
	\end{aligned}
	$
	\item 
	\! If $A$ is contained in $B$, then $P(A) \leq P(B)$.
	\item  
	\! 
	$
		\begin{aligned}
			P(A+B) + P(\bar A) + P(\bar B) - P(\bar A + \bar B) = 1 \nonumber
		\end{aligned}
	$ 
	\item
	\!  
	$
		\begin{aligned}
			P(AB) + P(\bar A C) + P(\bar B \bar C) \leq 1 \nonumber
		\end{aligned}
	$ \\[5pt]
	Please also give an example showing that the bound can be achieved.
\end{enumerate}

\subsection{Solution}

\begin{enumerate}[a.]
	\item To Prove: $P(A \bar{B}) = P(A) - P(AB)$
		\!
		\begin{proof}
			\begin{align}
				& \text{From the Law of Total Probability, we know that } \nonumber\\ 
				& \quad P(A) = P(A \bar{B}) + P(AB) \label{eq:totalProbLaw} \\
				& \text{Rearranging \cref{eq:totalProbLaw}, we get:} \nonumber\\
				& \quad P(A\bar{B}) = P(A) - P(AB) \\
				& \text{ Hence Proved. \Laughey[1.4]} \nonumber
			\end{align}
		\end{proof}
	\item To Prove: If $A$ is contained in $B$, then $P(A) \leq P(B)$
		\!
		\begin{proof}
			\begin{align}
				& \text{To Prove: } \text{if } A \subseteq B \text{,  then } P(A) \leq P(B) \nonumber \\
				& \text{From the Law of Total Probability, we know that} \nonumber\\
				& \quad P(B) = P(B\bar{A}) + P(BA) \label{eq:totalProbLawB}\\
				& \quad A \subseteq B \implies A \cap B = A \implies P(BA) = P(A) \nonumber\\
				& \quad \text{or,} \quad P(B) = P(B\bar{A}) + P(A) \nonumber\\
				& \text{But, by Axiom $1$ of Probability} \nonumber\\
				& \quad P(B\bar{A}) \geq 0 \nonumber\\
				& \quad \implies P(A) \leq P(B) \nonumber \\
				& \text{Hence Proved. \Laughey[1.4]} \nonumber			
			\end{align}
		\end{proof}
		\item \text{To Prove: } $P(A+B) + P(\bar A) + P(\bar B) - P(\bar A + \bar B) = 1$\\
		\!
			\begin{proof}
				\begin{align}
					LHS &= \{P(A) + P(B) - P(AB)\} + P(\bar{A}) + P(\bar{B}) &&\text{(Expanding the $LHS$)} \nonumber\\
					&- \{P(\bar{A}) + P(\bar{B}) - P(\bar{A}\bar{B})\}  \nonumber\\
					&= P(A) + P(B) - P(AB) + P(\bar{A}\bar{B}) \nonumber\\
					&= P(A) - P(AB) + P(\bar{A}\bar{B}) + P(B)&& \text{(Rearranging the equation)}\nonumber\\
					&= P(A\bar{B}) + P(\bar{A}\bar{B}) + P(B) &&\text{(Using \cref{eq:totalProbLaw})} \nonumber\\
					&= P(\bar{B}) + P(B) &&\text{(Using \cref{eq:totalProbLawB})} \nonumber\\
					&= 1 &&\text{Hence Proved \Laughey[1.4]}\nonumber
				\end{align}
			\end{proof}	
%			\text{Expanding the $LHS$:} \\
%			\begin{align}
%				&\quad LHS &= \{P(A) + P(B) - P(AB)\} + P(\bar{A}) + P(\bar{B}) \nonumber\\
%				& &\quad - \{P(\bar{A}) + P(\bar{B}) - P(\bar{A}\bar{B})\} \nonumber\\
%			\end{align}	
%			\begin{align}
%				&\quad LHS &= P(A) + P(B) - P(AB) + P(\bar{A}\bar{B}) \nonumber\\
%			\end{align}	
%	
%			\text{Rearranging the equation, we get:}\\
%			
%			\begin{align}
%				&\quad LHS &= P(A) - P(AB) + P(B) + P(\bar{A}\bar{B}) \nonumber\\
%			\end{align}
%				
%			\text{Using \cref{eq:totalProbLaw}, we get:}\\
%			
%			\begin{align}
%				&\quad LHS &= P(A\bar{B}) + P(B) + P(\bar{A}\bar{B}) \nonumber\\
%			\end{align}
%		
%			\text{Rearranging the equation, we get:}\\
%			\begin{align}
%				LHS &= P(A\bar{B}) + P(\bar{A}\bar{B}) + P(B) 
%			\end{align}
			
\end{enumerate}